chore: new rounder (#31)
* feat: add rounder

This implements unpacked float rounding.
We create many layers of helpful definitions,
to create the masks necessary for extracting guard, sticky, and
significand bits.

* chore: undo all changes to division file

* chore: cleanup file

* chore: add test against fixed point rounding

* chore: error: (978 succeeded / 992 total) (98.588710% succeeded) (14 failures)

* chore: success on E5M5 -> E5M2 rounding

* chore: fix late underflow circuit.

Recall that we late underflow when 'exp = minSubnormalExp - 1',
so it is possible for us to get back into representable range by
rounding up, but we fail to do so. (if exp < minSubnormalExp - 1, then
we early underflow).

* chore: add tests

* chore: cleanup

Fp/Basic.lean
@@ -25,7 +25,7 @@ structure PackedFloat (exWidth sigWidth : Nat) where
     ex : BitVec exWidth
     /-- Significand (mantissa) of the packed float. -/
     sig : BitVec sigWidth
-deriving DecidableEq, Repr
+deriving DecidableEq, Repr, Inhabited
 
 attribute [bv_normalize] PackedFloat.ext_iff
 
@@ -738,7 +738,7 @@ manipulation.
 structure EUnpackedFloat (e s : Nat) where
   state : State
   num   : UnpackedFloat e s
-deriving DecidableEq
+deriving DecidableEq, Repr
 
 inductive ExtDyadic where
   | NaN : ExtDyadic
@@ -750,7 +750,7 @@ inductive ExtRat where
   | NaN : ExtRat
   | Infinity : Bool → ExtRat
   | Number : Rat → ExtRat
-deriving DecidableEq
+deriving DecidableEq, Repr
 
 def ExtDyadic.toExtRat (ed : ExtDyadic) : ExtRat :=
   match ed with
@@ -889,6 +889,7 @@ theorem eq_num_ex {x y : EUnpackedFloat e s} :
   cases b <;> rfl
 
 
+
 @[bv_normalize]
 def isNaN (x : EUnpackedFloat e s) : Bool :=
   x.state == .NaN
@@ -986,9 +987,25 @@ def Nat.ceilLog2 (n : Nat) : Nat :=
 def minNormalExp (e : Nat) : Int :=
   -(bias e - 1 : Nat)
 
+/-- The max value the exponent can take when unbiased. -/
+@[bv_normalize]
+def maxNormalExp (e : Nat) : Int := (bias e)
+
+
+/-- The value the subnormal exponent can take. -/
+@[bv_normalize]
+def subnormalExp (e : Nat) : Int :=
+  minNormalExp e - 1
+
+/-- For unpacked floats, the *minimum* the subnormal exponent can take,
+which can "steal" bits from the significand to be smaller than minNormalExp. -/
+@[bv_normalize]
+def minSubnormalExp (e : Nat) (s : Nat) : Int :=
+  (subnormalExp e) - (s : Int)
+
 -- This is a simpler (but less tight) bound than `exponentWidth`.
 -- It's logarithmically larger.
-@[bv_normalize]
+@[bv_normalize, simp]
 def exponentWidth' (e s : Nat) : Nat :=
   e + s.ceilLog2
 
